\section{Resolution in FOL}
\begin{large}
    \textbf{Using resolution, prove the conclusions from Arguments A and B from exercise 3.}
    \subsection{Argument A}
    \begin{enumerate}
        \item $\mathbf{\forall x : [flies(x, Robinson) \rightarrow Pitcher(x)]}$
        \item $\mathbf{scores(Crabb) \rightarrow (flies(Samson, Robinson) \land Centerfielder(Robinson))}$
        \item $\mathbf{scores(Crabb)}$
    \end{enumerate}
    Proof by contradiction\@: $\neg Pitcher(Samson)$.

    Insert (2) into (3):

    (4) $ scores(Crabb) \rightarrow (flies(Samson, Robinson) \land Centerfielder(Robinson)) $

    Replace x with Samson in (1):

    (5) $flies(Samson, Robinson) \rightarrow Pitcher(Samson)$

    As we assume $\neg Pitcher(Samson)$, (5) must be false.

    Therefore $flies(Samson, Robinson)$ must be false.
    Consequently, the right hand side of (4) must also be false.

    Thus, we have proven by contradiction\@: $ Pitcher(Samson)$.

    \subsection{Argument B}

    \begin{enumerate}
        \item $\mathbf{\forall x : [(Centerfielder(x) \land \neg scores(x)) \rightarrow \neg \exists y : [friend(y, x)]]}$
        \item $\mathbf{Centerfielder(Robinson) \land Centerfielder(Jones)}$
        \item $\mathbf{\forall x : [(Centerfielder(x) \land flies(x, Jones)) \rightarrow \neg scores(x)]}$
        \item $\mathbf{flies(Robinson, Jones)}$
    \end{enumerate}
    Proof by contradiction\@: $friend(Jones, Robinson)$.

    By combining (3) and (4), thus replacing x with Robinson, we get:
    $(Centerfielder(Robinson) \land flies(Robinson, Jones)) \rightarrow \neg scores(Robinson)$

    Thus we get that Robinson is centerfield and doesn't score. By inserting this into (1), we get:

    (5) $(Centerfielder(Robinson) \land \neg scores(Robinson)) \rightarrow \neg \exists y : [friend(y, Robinson)]$

    As y can be any person, we can insert Jones into (5), which gives $\neg friend(Jones, Robinson)$.
    This is a contradiction to what we desired to prove, thus $friend(Jones, Robinson)$ must be false.
\end{large}